TypeTheorems.thy
@@ -1,5 +1,46 @@
 theory TypeTheorems imports gASPFuturesTypeSystem begin
 
+section{* Induction lemmas *}
+lemma TypeExpression_induct_Config:
+"P,Cn aos futs,\<Gamma> in C\<turnstile>\<^sub>Ee:T \<Longrightarrow>
+    (\<And>P aos futs \<Gamma> C v T. P,Cn aos futs,\<Gamma> in C\<turnstile>\<^sub>Av:T \<Longrightarrow> Prop P aos futs \<Gamma> C (At v) T) \<Longrightarrow>
+    (\<And>P aos futs \<Gamma> C e e'. P,Cn aos futs,\<Gamma> in C\<turnstile>\<^sub>Ae:BType Integer \<Longrightarrow> P,Cn aos futs,\<Gamma> in C\<turnstile>\<^sub>Ae':BType Integer \<Longrightarrow> Prop P aos futs \<Gamma> C (e+\<^sub>Ae') (BType Integer)) \<Longrightarrow> 
+    (\<And>P T T' aos futs \<Gamma> C e.  P\<turnstile>T\<sqsubseteq>T' \<Longrightarrow> P,Cn aos futs,\<Gamma> in C\<turnstile>\<^sub>Ee:T \<Longrightarrow> Prop P aos futs \<Gamma> C e T \<Longrightarrow>Prop P  aos futs \<Gamma> C e T') 
+          \<Longrightarrow> Prop P aos futs  \<Gamma> C e T"
+apply (insert gASPFuturesTypeSystem.TypeExpression.induct [of  P "Cn aos futs" \<Gamma> C e T  "\<lambda> x conf y z t. (Prop x (Conf_AOs conf) (Conf_futs conf) y z t)" ])
+apply clarsimp
+ apply (drule meta_impE,auto,case_tac Config,auto)+
+done
+
+lemma TypeStatement_TypeStatementList_induct_Config:
+"  (\<And>P aos futs \<Gamma> C a T x T'. P,Cn aos futs,\<Gamma> in C\<turnstile>\<^sub>Ra:T \<Longrightarrow> \<Gamma> x = Some T' \<Longrightarrow>  P\<turnstile>T\<sqsubseteq>T' \<Longrightarrow> P1 P aos futs \<Gamma> C (x =\<^sub>A a)) \<Longrightarrow>
+    (\<And>P C Class m Meth T' aos futs \<Gamma> e T x. fetchClass P C = Some Class \<Longrightarrow> fetchMethodInClass Class m = Some Meth \<Longrightarrow> MRType Meth = T' \<Longrightarrow> P,Cn aos futs,\<Gamma> in C\<turnstile>\<^sub>Ee:T \<Longrightarrow> \<Gamma> x = Some T' \<Longrightarrow>  P\<turnstile>T\<sqsubseteq>T' \<Longrightarrow> P1 P aos futs \<Gamma> C (return e)) \<Longrightarrow>
+    (\<And>P aos futs \<Gamma> C z  sl sl'. P,Cn aos futs,\<Gamma> in C\<turnstile>\<^sub>Az:BType Boolean \<Longrightarrow> (P,Cn aos futs,\<Gamma> in C\<turnstile>\<^sub>L sl)  \<Longrightarrow> P2 P aos futs \<Gamma> C sl \<Longrightarrow> P,Cn aos futs,\<Gamma> in C\<turnstile>\<^sub>L sl'  \<Longrightarrow> P2 P aos futs \<Gamma> C sl' \<Longrightarrow> P1 P aos futs \<Gamma> C (IF z THEN sl ELSE sl' )) \<Longrightarrow>
+    (\<And>P aos futs \<Gamma> C. P2 P aos futs \<Gamma> C []) \<Longrightarrow>
+    (\<And>P aos futs \<Gamma> C s sl. P,Cn aos futs,\<Gamma> in C\<turnstile>\<^sub>S s  \<Longrightarrow> P1 P aos futs \<Gamma> C s \<Longrightarrow> P,Cn aos futs,\<Gamma> in C\<turnstile>\<^sub>L sl  \<Longrightarrow> P2 P aos futs \<Gamma> C sl \<Longrightarrow> P2 P aos futs \<Gamma> C (s ;; sl)) \<Longrightarrow>
+    ((P,Cn aos futs,\<Gamma> in x4\<turnstile>\<^sub>S x5)  \<longrightarrow> P1 P aos futs \<Gamma> x4 x5) \<and> ((P',Cn aos' futs',\<Gamma>' in x9\<turnstile>\<^sub>L x10)  \<longrightarrow> P2 P' aos' futs' \<Gamma>'  x9 x10)"
+apply (insert gASPFuturesTypeSystem.TypeStatement_TypeStatementList.induct [of "\<lambda> x conf y z t. (P1 x (Conf_AOs conf) (Conf_futs conf) y z t)" "\<lambda> x conf y z t. (P2 x (Conf_AOs conf) (Conf_futs conf) y z t)" P "Cn aos futs" \<Gamma> x4 x5 P' "Cn aos' futs'" \<Gamma>' x9 x10])
+apply rule
+ apply (drule meta_impE,auto,case_tac Config,auto)+
+done
+
+lemma TypeRhs_induct_Config:
+"(P,Cn aos futs,\<Gamma> in C\<turnstile>\<^sub>RR: T)\<Longrightarrow>
+    (\<And>P aos futs \<Gamma> C e T. (P,Cn aos futs,\<Gamma> in C\<turnstile>\<^sub>Ee:T) \<Longrightarrow> P1 P aos futs \<Gamma> C (Expr e) T) \<Longrightarrow>
+    (\<And>P aos futs \<Gamma> C z C' Class m Meth param_types el.
+        (P,Cn aos futs,\<Gamma> in C\<turnstile>\<^sub>Az:BType (TObj C')) \<Longrightarrow>
+        fetchClass P C' = Some Class \<Longrightarrow> fetchMethodInClass Class m = Some Meth \<Longrightarrow> param_types = map fst (MParams Meth) \<Longrightarrow> length param_types = length el \<Longrightarrow> \<forall>i<length el. (P,Cn aos futs,\<Gamma> in C\<turnstile>\<^sub>Eel ! i:param_types ! i) 
+                  \<Longrightarrow> P1 P  aos futs \<Gamma> C (z.\<^sub>Am(el)) (MakeFutureType (MRType Meth))) \<Longrightarrow>
+    (\<And>P C' Class Class_param_types el aos futs \<Gamma> C. fetchClass P C' = Some Class \<Longrightarrow> Class_param_types = map fst (ClassParameters Class) \<Longrightarrow> length Class_param_types = length el 
+                  \<Longrightarrow> \<forall>i<length el. (P,Cn aos futs,\<Gamma> in C\<turnstile>\<^sub>E(el ! i):(Class_param_types ! i)) \<Longrightarrow> P1 P  aos futs \<Gamma> C (newActive C'(el)) (BType (TObj C'))) \<Longrightarrow>
+    (\<And>P aos futs \<Gamma> C z T. (P,Cn aos futs,\<Gamma> in C\<turnstile>\<^sub>Az:FutType T) \<Longrightarrow> P1 P  aos futs \<Gamma> C (Get z) (BType T)) \<Longrightarrow> (\<And>P T T'  aos futs \<Gamma> C e.  P\<turnstile>T\<sqsubseteq>T' 
+                  \<Longrightarrow> P,Cn aos futs,\<Gamma> in C\<turnstile>\<^sub>Re:T \<Longrightarrow> P1 P  aos futs \<Gamma> C e T \<Longrightarrow> P1 P aos futs \<Gamma> C e T') 
+\<Longrightarrow> P1 P aos futs \<Gamma> C R T"
+apply (insert TypeRhs.induct [of  P "Cn aos futs" \<Gamma> C R T "\<lambda> x conf y z t. (P1 x (Conf_AOs conf) (Conf_futs conf) y z t)"])
+apply auto
+apply (drule meta_impE,auto,case_tac Config,auto)+
+done
+
 section{* Basic Lemmas *}
 
 lemma TypeStatementList_TypeStatement[rule_format]: 
@@ -9,31 +50,9 @@ apply (induct_tac Stl)
 apply (drule TypeStatementList.cases,auto)
 done
 
-lemma TypeStatement_TypeStatementList_induct_Config:
-"  (\<And>P aos futs \<Gamma> C a T x T'. P,Cn aos futs,\<Gamma> in C\<turnstile>\<^sub>Ra:T \<Longrightarrow> \<Gamma> x = Some T' \<Longrightarrow>  P\<turnstile>T\<sqsubseteq>T' \<Longrightarrow> P1 P aos futs \<Gamma> C (x =\<^sub>A a)) \<Longrightarrow>
-    (\<And>P C Class m Meth T' aos futs \<Gamma> e T x. fetchClass P C = Some Class \<Longrightarrow> fetchMethodInClass Class m = Some Meth \<Longrightarrow> MRType Meth = T' \<Longrightarrow> P,Cn aos futs,\<Gamma> in C\<turnstile>\<^sub>Ee:T \<Longrightarrow> \<Gamma> x = Some T' \<Longrightarrow>  P\<turnstile>T\<sqsubseteq>T' \<Longrightarrow> P1 P aos futs \<Gamma> C (return e)) \<Longrightarrow>
-    (\<And>P aos futs \<Gamma> C e  sl sl'. P,Cn aos futs,\<Gamma> in C\<turnstile>\<^sub>Ee:BType Boolean \<Longrightarrow> P,Cn aos futs,\<Gamma> in C\<turnstile>\<^sub>L sl  \<Longrightarrow> P2 P aos futs \<Gamma> C sl \<Longrightarrow> P,Cn aos futs,\<Gamma> in C\<turnstile>\<^sub>L sl'  \<Longrightarrow> P2 P aos futs \<Gamma> C sl' \<Longrightarrow> P1 P aos futs \<Gamma> C (IF e THEN sl ELSE sl' )) \<Longrightarrow>
-    (\<And>P aos futs \<Gamma> C. P2 P aos futs \<Gamma> C []) \<Longrightarrow>
-    (\<And>P aos futs \<Gamma> C s sl. P,Cn aos futs,\<Gamma> in C\<turnstile>\<^sub>S s  \<Longrightarrow> P1 P aos futs \<Gamma> C s \<Longrightarrow> P,Cn aos futs,\<Gamma> in C\<turnstile>\<^sub>L sl  \<Longrightarrow> P2 P aos futs \<Gamma> C sl \<Longrightarrow> P2 P aos futs \<Gamma> C (s ;; sl)) \<Longrightarrow>
-    (P,Cn aos futs,\<Gamma> in x4\<turnstile>\<^sub>S x5  \<longrightarrow> P1 P aos futs \<Gamma> x4 x5) \<and> (P',Cn aos' futs',\<Gamma>' in x9\<turnstile>\<^sub>L x10  \<longrightarrow> P2 P' aos' futs' \<Gamma>'  x9 x10)"
-apply (insert gASPFuturesTypeSystem.TypeStatement_TypeStatementList.induct [of "\<lambda> x conf y z t. (P1 x (Conf_AOs conf) (Conf_futs conf) y z t)" "\<lambda> x conf y z t. (P2 x (Conf_AOs conf) (Conf_futs conf) y z t)" P "Cn aos futs" \<Gamma> x4 x5 P' "Cn aos' futs'" \<Gamma>' x9 x10])
-apply rule
- apply (drule meta_impE,auto,case_tac Config,auto)+
-done
 
-lemma TypeRhs_induct_Config:
-"(P,Cn aos futs,\<Gamma> in C\<turnstile>\<^sub>RR: T)\<Longrightarrow>
-    (\<And>P aos futs \<Gamma> C e T. (P,Cn aos futs,\<Gamma> in C\<turnstile>\<^sub>Ee:T) \<Longrightarrow> P1 P aos futs \<Gamma> C (Expr e) T) \<Longrightarrow>
-    (\<And>P aos futs \<Gamma> C e C' Class m Meth param_types el.
-        (P,Cn aos futs,\<Gamma> in C\<turnstile>\<^sub>Ee:BType (TObj C')) \<Longrightarrow>
-        fetchClass P C' = Some Class \<Longrightarrow> fetchMethodInClass Class m = Some Meth \<Longrightarrow> param_types = map fst (MParams Meth) \<Longrightarrow> length param_types = length el \<Longrightarrow> \<forall>i<length el. (P,Cn aos futs,\<Gamma> in C\<turnstile>\<^sub>Eel ! i:param_types ! i) \<Longrightarrow> P1 P  aos futs \<Gamma> C (e.\<^sub>Am(el)) (MakeFutureType (MRType Meth))) \<Longrightarrow>
-    (\<And>P C' Class Class_param_types el aos futs \<Gamma> C. fetchClass P C' = Some Class \<Longrightarrow> Class_param_types = map fst (ClassParameters Class) \<Longrightarrow> length Class_param_types = length el \<Longrightarrow> \<forall>i<length el. (P,Cn aos futs,\<Gamma> in C\<turnstile>\<^sub>E(el ! i):(Class_param_types ! i)) \<Longrightarrow> P1 P  aos futs \<Gamma> C (newActive C'(el)) (BType (TObj C'))) \<Longrightarrow>
-    (\<And>P aos futs \<Gamma> C e T. (P,Cn aos futs,\<Gamma> in C\<turnstile>\<^sub>Ee:FutType T) \<Longrightarrow> P1 P  aos futs \<Gamma> C (Get e) (BType T)) \<Longrightarrow> (\<And>P T T'  aos futs \<Gamma> C e.  P\<turnstile>T\<sqsubseteq>T' \<Longrightarrow> P,Cn aos futs,\<Gamma> in C\<turnstile>\<^sub>Re:T \<Longrightarrow> P1 P  aos futs \<Gamma> C e T \<Longrightarrow> P1 P aos futs \<Gamma> C e T') 
-\<Longrightarrow> P1 P aos futs \<Gamma> C R T"
-apply (insert TypeRhs.induct [of  P "Cn aos futs" \<Gamma> C R T "\<lambda> x conf y z t. (P1 x (Conf_AOs conf) (Conf_futs conf) y z t)"])
-apply auto
-apply (drule meta_impE,auto,case_tac Config,auto)+
-done
+section{* extending set of AOs in config *}
+
 lemma TypeValue_extendconfiguration_AO[rule_format]:
 "P,Cn AOs Futures\<turnstile>\<^sub>Vv:T \<Longrightarrow> (case AOs \<alpha> of Some (AO C' st' R' Ec' Rq') \<Rightarrow> C=C' | None \<Rightarrow> True) \<Longrightarrow>(P,Cn (AOs(\<alpha> \<mapsto> AO C state R Ec Rq)) Futures\<turnstile>\<^sub>Vv:T)"
 apply (erule TypeValue.cases,auto)
@@ -46,21 +65,31 @@ apply (erule TypeValue.cases,auto)
 apply (rule TypeValue.intros,force)
 done
 
-lemma TypeExpression_extendconfiguration_AO[rule_format]:
-"P,Cn aos futs,\<Gamma> in C\<turnstile>\<^sub>Ee:T \<Longrightarrow> (aos \<alpha> = None \<longrightarrow> (futs f = None\<longrightarrow>( P,Cn (\<lambda>a. if a = \<alpha> then Some X else AOs a) (\<lambda>a. if a = f then Some Y else futs a),\<Gamma> in C\<turnstile>\<^sub>Ee:T)))"
-apply (erule  "TypeExpression.induct",auto)
+lemma TypeAtom_extendconfiguration_AO[rule_format]:
+"P,Cn aos futs,\<Gamma> in C\<turnstile>\<^sub>Az:T \<Longrightarrow> (aos \<alpha> = None \<longrightarrow> ( P,Cn (\<lambda>a. if a = \<alpha> then Some X else aos a)  futs ,\<Gamma> in C\<turnstile>\<^sub>Az:T))"
+apply (erule  "TypeAtom.induct",auto)
     apply (rule  "TypeValue.cases",auto)
-        apply (rule  "TypeExpression.intros",(auto)?)+
+        apply (rule  "TypeAtom.intros",(auto)?)+
+done
+lemma TypeExpression_extendconfiguration_AO[rule_format]:
+"P,Cn aos futs,\<Gamma> in C\<turnstile>\<^sub>Ee:T \<Longrightarrow> (aos \<alpha> = None \<longrightarrow> ( P,Cn (\<lambda>a. if a = \<alpha> then Some X else aos a)  futs ,\<Gamma> in C\<turnstile>\<^sub>Ee:T))"
+apply (erule  "TypeExpression_induct_Config",auto)
+  apply (rule  "TypeExpression.intros",(auto)?)+
+  apply (rule  "TypeAtom_extendconfiguration_AO",auto)
+ apply (rule  "TypeExpression.intros",(auto)?)+
+  apply (rule  "TypeAtom_extendconfiguration_AO",auto)
+ apply (rule  "TypeAtom_extendconfiguration_AO",auto)
+apply (rule  "TypeExpression.intros",auto)
 done
 
 lemma TypeRhs_extendconfiguration_AO[rule_format]:
-"P,Cn aos futs,\<Gamma> in C\<turnstile>\<^sub>Ra:T \<Longrightarrow> (aos \<alpha> = None \<longrightarrow> (futs f = None\<longrightarrow>(P,Cn (\<lambda>a. if a = \<alpha> then Some X else AOs a) (\<lambda>a. if a = f then Some Y else futs a),\<Gamma> in C\<turnstile>\<^sub>Ra:T)))"
+"P,Cn aos futs,\<Gamma> in C\<turnstile>\<^sub>Ra:T \<Longrightarrow> (aos \<alpha> = None \<longrightarrow>(P,Cn (\<lambda>a. if a = \<alpha> then Some X else aos a) futs,\<Gamma> in C\<turnstile>\<^sub>Ra:T))"
 apply (erule  "TypeRhs_induct_Config",auto)
 (*5*)
     apply (rule  "TypeRhs.intros",(auto)?)
     apply (erule TypeExpression_extendconfiguration_AO,auto)
    apply (rule  "TypeRhs.intros",(auto)?)
-    apply (erule TypeExpression_extendconfiguration_AO,auto)
+    apply (erule TypeAtom_extendconfiguration_AO,auto)
    apply (rule_tac aos=aos in TypeExpression_extendconfiguration_AO)
      apply (drule_tac x=i in spec,auto)
 (*3*)
@@ -68,46 +97,120 @@ apply (erule  "TypeRhs_induct_Config",auto)
   apply (rule_tac aos=aos in TypeExpression_extendconfiguration_AO)
     apply (drule_tac x=i in spec,auto)
  apply (rule  "TypeRhs.intros",(auto)?)
- apply (erule TypeExpression_extendconfiguration_AO,force,force)
+ apply (erule TypeAtom_extendconfiguration_AO,force)
 apply (rule  "TypeRhs.intros",(auto)?)
 done
 
+
 lemma TypeStatement_extendconfiguration_AO_Pre[rule_format]:
-" ((P,Cn AOs futs,\<Gamma> in C \<turnstile>\<^sub>S S) \<longrightarrow> (\<forall> \<alpha> X. \<alpha>\<notin>(dom AOs)\<longrightarrow>(\<forall> f Y. f\<notin>(dom futs)\<longrightarrow> (P, Cn (AOs(\<alpha>\<mapsto>X)) (futs(f\<mapsto>Y)),\<Gamma> in C \<turnstile>\<^sub>S S)))) \<and> 
-  ((P, Cn AOs futs,\<Gamma> in C \<turnstile>\<^sub>L Stl) \<longrightarrow> (\<forall> \<alpha> X. \<alpha>\<notin>(dom AOs)\<longrightarrow>(\<forall> f Y. f\<notin>(dom futs)\<longrightarrow> (P, Cn (AOs(\<alpha>\<mapsto>X)) (futs(f\<mapsto>Y)),\<Gamma> in C \<turnstile>\<^sub>L Stl))))"
+" ((P,Cn AOs futs,\<Gamma> in C \<turnstile>\<^sub>S S) \<longrightarrow> (\<forall> \<alpha> X. \<alpha>\<notin>(dom AOs)\<longrightarrow> (P, Cn (AOs(\<alpha>\<mapsto>X)) futs,\<Gamma> in C \<turnstile>\<^sub>S S))) \<and> 
+  ((P, Cn AOs futs,\<Gamma> in C \<turnstile>\<^sub>L Stl) \<longrightarrow> (\<forall> \<alpha> X. \<alpha>\<notin>(dom AOs)\<longrightarrow> (P, Cn (AOs(\<alpha>\<mapsto>X)) futs,\<Gamma> in C \<turnstile>\<^sub>L Stl)))"
 apply (rule TypeStatement_TypeStatementList_induct_Config,auto)
 (*5*)
     apply (rule  "TypeStatement_TypeStatementList.intros",auto)
     apply (erule TypeRhs_extendconfiguration_AO,auto)
-    apply (rotate_tac -1,erule contrapos_pp,force)  
    apply (rule  "TypeStatement_TypeStatementList.intros",auto)
    apply (erule TypeExpression_extendconfiguration_AO,auto)
-   apply (rotate_tac -1,erule contrapos_pp,force)
   apply (rule  "TypeStatement_TypeStatementList.intros")
 (*5*)
-    apply (erule TypeExpression_extendconfiguration_AO,auto)
-    apply (rotate_tac -1,erule contrapos_pp,force)
-   apply (drule_tac x=\<alpha> in spec)+
-   apply force
-  apply (drule_tac x=\<alpha> in spec)+
-  apply force
+    apply (erule TypeAtom_extendconfiguration_AO,auto)
  apply (rule  "TypeStatement_TypeStatementList.intros")
 apply (rule  "TypeStatement_TypeStatementList.intros")
- apply (drule_tac x=\<alpha> in spec)+
- apply force
-apply (drule_tac x=\<alpha> in spec)+
-apply force
+ apply auto
 done
 
+(* GLOBAL LEMMAS *)
 lemma TypeStatement_extendconfiguration_AO:
-" (P,Cn AOs futs,\<Gamma> in C \<turnstile>\<^sub>S S) \<Longrightarrow> \<alpha>\<notin>dom AOs \<Longrightarrow>f\<notin> dom futs \<Longrightarrow> (P, Cn (AOs(\<alpha>\<mapsto>X)) (futs(f\<mapsto>Y)),\<Gamma> in C \<turnstile>\<^sub>S S) "
-by (case_tac Y,insert TypeStatement_extendconfiguration_AO_Pre,auto)
+" (P,Cn AOs futs,\<Gamma> in C \<turnstile>\<^sub>S S) \<Longrightarrow>\<alpha>\<notin>(dom AOs) \<Longrightarrow>P, Cn (AOs(\<alpha>\<mapsto>X)) futs,\<Gamma> in C \<turnstile>\<^sub>S S"
+by (insert TypeStatement_extendconfiguration_AO_Pre, auto)
 
 lemma TypeStatementList_extendconfiguration_AO:
-" (P,Cn AOs futs,\<Gamma> in C \<turnstile>\<^sub>L Stl) \<Longrightarrow> \<alpha>\<notin>(dom AOs) \<Longrightarrow>f\<notin> dom futs \<Longrightarrow> (P, Cn (AOs(\<alpha>\<mapsto>X)) (futs(f\<mapsto>Y)),\<Gamma> in C \<turnstile>\<^sub>L Stl) "
-by (case_tac Y,insert TypeStatement_extendconfiguration_AO_Pre,auto)
+" (P,Cn AOs futs,\<Gamma> in C \<turnstile>\<^sub>L Stl) \<Longrightarrow>\<alpha>\<notin>(dom AOs) \<Longrightarrow>P, Cn (AOs(\<alpha>\<mapsto>X)) futs,\<Gamma> in C \<turnstile>\<^sub>L Stl"
+by (insert TypeStatement_extendconfiguration_AO_Pre, auto)
+
+section{* extending set of futs in config *}
+
+lemma TypeAtom_extendconfiguration_futs[rule_format]:
+"P,Cn aos futs,\<Gamma> in C\<turnstile>\<^sub>Az:T \<Longrightarrow> futs f = None\<longrightarrow>( P,Cn aos (\<lambda>a. if a = f then Some Y else futs a),\<Gamma> in C\<turnstile>\<^sub>Az:T)"
+apply (erule  "TypeAtom.induct",auto)
+    apply (rule  "TypeValue.cases",auto)
+        apply (rule  "TypeAtom.intros",(auto)?)+
+done
+lemma TypeExpression_extendconfiguration_futs[rule_format]:
+"P,Cn aos futs,\<Gamma> in C\<turnstile>\<^sub>Ee:T \<Longrightarrow> futs f = None\<longrightarrow>( P,Cn aos (\<lambda>a. if a = f then Some Y else futs a),\<Gamma> in C\<turnstile>\<^sub>Ee:T)"
+apply (erule  "TypeExpression_induct_Config",auto)
+  apply (rule  "TypeExpression.intros",(auto)?)+
+  apply (rule  "TypeAtom_extendconfiguration_futs",auto)
+ apply (rule  "TypeExpression.intros",(auto)?)+
+  apply (rule  "TypeAtom_extendconfiguration_futs",auto)
+ apply (rule  "TypeAtom_extendconfiguration_futs",auto)
+apply (rule  "TypeExpression.intros",auto)
+done
+
+
+lemma TypeRhs_extendconfiguration_futs[rule_format]:
+"P,Cn aos futs,\<Gamma> in C\<turnstile>\<^sub>Ra:T \<Longrightarrow> (futs f = None\<longrightarrow>(P,Cn aos (\<lambda>a. if a = f then Some Y else futs a),\<Gamma> in C\<turnstile>\<^sub>Ra:T))"
+apply (erule  "TypeRhs_induct_Config",auto)
+(*5*)
+    apply (rule  "TypeRhs.intros",(auto)?)
+    apply (erule TypeExpression_extendconfiguration_futs,auto)
+   apply (rule  "TypeRhs.intros",(auto)?)
+    apply (erule TypeAtom_extendconfiguration_futs,auto)
+   apply (rule_tac aos=aos in TypeExpression_extendconfiguration_futs)
+     apply (drule_tac x=i in spec,auto)
+(*3*)
+  apply (rule  "TypeRhs.intros",(auto)?)
+  apply (rule_tac aos=aos in TypeExpression_extendconfiguration_futs)
+    apply (drule_tac x=i in spec,auto)
+ apply (rule  "TypeRhs.intros",(auto)?)
+ apply (erule TypeAtom_extendconfiguration_futs,force)
+apply (rule  "TypeRhs.intros",(auto)?)
+done
+
+lemma TypeStatement_extendconfiguration_futs_Pre[rule_format]:
+" ((P,Cn AOs futs,\<Gamma> in C \<turnstile>\<^sub>S S) \<longrightarrow> (\<forall> f Y. f\<notin>(dom futs)\<longrightarrow> (P, Cn AOs (futs(f\<mapsto>Y)),\<Gamma> in C \<turnstile>\<^sub>S S))) \<and> 
+  ((P, Cn AOs futs,\<Gamma> in C \<turnstile>\<^sub>L Stl) \<longrightarrow> (\<forall> f Y. f\<notin>(dom futs)\<longrightarrow> (P, Cn AOs (futs(f\<mapsto>Y)),\<Gamma> in C \<turnstile>\<^sub>L Stl)))"
+apply (rule TypeStatement_TypeStatementList_induct_Config,auto)
+(*5*)
+    apply (rule  "TypeStatement_TypeStatementList.intros",auto)
+    apply (erule TypeRhs_extendconfiguration_futs,auto)
+    apply (rotate_tac -1,erule contrapos_pp,force)  
+   apply (rule  "TypeStatement_TypeStatementList.intros",auto)
+   apply (erule TypeExpression_extendconfiguration_futs,auto)
+    apply (rotate_tac -1,erule contrapos_pp,force)  
+  apply (rule  "TypeStatement_TypeStatementList.intros")
+(*5*)
+    apply (erule TypeAtom_extendconfiguration_futs,auto)
+    apply (rotate_tac -1,erule contrapos_pp,force)
+   apply (drule_tac x=f in spec,auto)+
+ apply (rule  "TypeStatement_TypeStatementList.intros")
+apply (rule  "TypeStatement_TypeStatementList.intros")
+ apply (drule_tac x=f in spec,auto)+
+done
+
+(* GLOBAL LEMMAS *)
+lemma TypeStatement_extendconfiguration_futs:
+" (P,Cn AOs futs,\<Gamma> in C \<turnstile>\<^sub>S S) \<Longrightarrow>f\<notin>(dom futs) \<Longrightarrow>P, Cn AOs (futs(f\<mapsto>Y)),\<Gamma> in C \<turnstile>\<^sub>S S"
+by (insert TypeStatement_extendconfiguration_futs_Pre,case_tac Y, simp)
+
+lemma TypeStatementList_extendconfiguration_futs:
+" (P,Cn AOs futs,\<Gamma> in C \<turnstile>\<^sub>L Stl) \<Longrightarrow>f\<notin>(dom futs) \<Longrightarrow>P, Cn AOs (futs(f\<mapsto>Y)),\<Gamma> in C \<turnstile>\<^sub>L Stl"
+by (insert TypeStatement_extendconfiguration_futs_Pre,case_tac Y, simp)
+
+
+section {* extend AOs and futs *}
+lemma TypeStatement_extendconfiguration:
+" (P,Cn AOs futs,\<Gamma> in C \<turnstile>\<^sub>S S) \<Longrightarrow>\<alpha>\<notin>dom AOs \<Longrightarrow>f\<notin>(dom futs) \<Longrightarrow>P, Cn (AOs(\<alpha>\<mapsto>X)) (futs(f\<mapsto>Y)),\<Gamma> in C \<turnstile>\<^sub>S S"
+by (insert TypeStatement_extendconfiguration_futs,insert TypeStatement_extendconfiguration_AO, auto)
+
+lemma TypeStatementList_extendconfiguration:
+" (P,Cn AOs futs,\<Gamma> in C \<turnstile>\<^sub>L Stl) \<Longrightarrow>\<alpha>\<notin>dom AOs \<Longrightarrow>f\<notin>(dom futs) \<Longrightarrow>P, Cn (AOs(\<alpha>\<mapsto>X)) (futs(f\<mapsto>Y)),\<Gamma> in C \<turnstile>\<^sub>L Stl"
+by (insert TypeStatementList_extendconfiguration_futs,insert TypeStatementList_extendconfiguration_AO, auto)
+
+section {* compositional lemmas for WT *}
 
 lemma TypeUpdate_AO:  "P \<turnstile> Cn AOs Futures  \<Longrightarrow>
+  (case AOs \<alpha> of Some (AO C' st' R' Ec' Rq') \<Rightarrow> C=C' | None \<Rightarrow> True) \<Longrightarrow>
    (\<exists> CL . (fetchClass P C = Some CL \<and>
     (
      (* check state *)
@@ -124,27 +227,47 @@ lemma TypeUpdate_AO:  "P \<turnstile> Cn AOs Futures  \<Longrightarrow>
         )) ) ) )))
 \<Longrightarrow> P \<turnstile> Cn (AOs(\<alpha> \<mapsto> AO C state R Ec Rq)) Futures "
 apply (clarsimp,auto)
-apply (case_tac "Act = AO C state R Ec Rq",clarsimp)
-apply (drule_tac x=Act in bspec)
-apply (clarsimp simp: ran_def)
-apply (case_tac "a = \<alpha>",simp,force)
-apply (case_tac Act,clarsimp)
-apply (intro allI conjI)
+  apply (clarsimp simp: ran_def)
+  apply (case_tac "a = \<alpha>",simp,force)
+apply clarsimp
+ apply (case_tac Act,clarsimp)
 
+apply (drule_tac x= "(AO x1 x2 x3 (aa, b) x5)" in spec)
+apply clarsimp
+apply (erule impE,force)
+apply clarsimp
+ apply (intro allI conjI)
 apply clarsimp
 apply (drule_tac x=x in spec)+
 apply (drule_tac x=v in spec)+
 apply clarsimp
-apply (erule gASPFuturesTypeSystem.TypeValue.cases)
+apply (rule_tac x=T in exI)
 apply clarsimp
-apply (rule_tac x="FutType T" in exI)
+apply (erule TypeValue_extendconfiguration_AO)
 apply clarsimp
-apply (rule gASPFuturesTypeSystem.TypeValue.intros(5))
 
+(*Q*)
+apply clarsimp
+apply (rename_tac a)
+(* one of the pending request *)
+apply (drule_tac x="(ab, ac, a)" in bspec,simp)
+apply (erule TypeRequest.cases)
+apply (rule_tac Meth=Meth in TypeRequest.intros)
+apply auto
+apply (drule_tac x=i in spec,clarsimp)
+apply (rule TypeValue_extendconfiguration_AO)
+apply clarsimp+
 
-apply (rule_tac  TypeStatementList_extendconfiguration_AO)
-apply for
-
+(* the current req*)
+apply (case_tac x3,auto)
+apply (erule TypeRequest.cases)
+apply (rule_tac Meth=Meth in TypeRequest.intros)
+apply auto
+apply (drule_tac x=i in spec,clarsimp)
+apply (rule TypeValue_extendconfiguration_AO)
+apply auto
+apply (drule_tac x=x in bspec,auto)
+apply (rule TypeStatement_extendconfiguration_AO)
 
 section{* Well-typed initial configuraiton *}
 
